cedar-lean/Cedar/Thm/TPE/Input.lean
@@ -17,15 +17,135 @@
 import Cedar.TPE.Input
 import Cedar.Spec
 import Cedar.Validation
+import Cedar.Thm
 
 namespace Cedar.Thm
 
 open Cedar.TPE
 open Cedar.Spec
 open Cedar.Validation
+open Cedar.Thm
+
+/-
+-- We do not check if `req`'s action is valid (i.e, if it's contained in `env`)
+-- because this function is called after validation, which already ensures it
+def requestIsValid (env : Environment) (req : PartialRequest) : Bool :=
+  (partialIsValid req.principal.asEntityUID λ principal =>
+    instanceOfEntityType principal principal.ty env.ets.entityTypeMembers?) &&
+  (partialIsValid req.resource.asEntityUID λ resource =>
+    instanceOfEntityType resource resource.ty env.ets.entityTypeMembers?) &&
+  (partialIsValid req.context λ m =>
+    instanceOfType (.record m) (.record env.reqty.context) env.ets)
+-/
+
+inductive PartialIsValid {α} : (α → Prop) → Option α -> Prop
+  | some (p : α → Prop) (x : α)
+    (h : p x) :
+    PartialIsValid p (.some x)
+  | none :
+    PartialIsValid p .none
+
+theorem partial_is_valid_rfl (f : α → Bool) (p : α → Prop) (o : Option α) :
+  (∀ x, f x = true → p x) → partialIsValid o f → PartialIsValid p o
+:= by
+  intro h₁
+  simp [partialIsValid, Option.map]
+  split <;> simp [Option.getD]
+  case _ x =>
+    intro h₂
+    constructor
+    exact h₁ x h₂
+  case _ =>
+    constructor
+
+def PartialRequestMatchesEnvironment (env : Environment) (request : PartialRequest) : Prop :=
+  PartialIsValid (InstanceOfEntityType · env.reqty.principal) request.principal.asEntityUID ∧
+  PartialIsValid (InstanceOfEntityType · env.reqty.resource) request.resource.asEntityUID ∧
+  PartialIsValid (InstanceOfType · (.record env.reqty.context)) request.context
+
+/-
+∀ uid data, entities.find? uid = some data →
+    ∃ entry, ets.find? uid.ty = some entry ∧
+      IsValidEntityEID entry uid.eid ∧
+      InstanceOfType data.attrs (.record entry.attrs) ∧
+      (∀ ancestor, ancestor ∈ data.ancestors → ancestor.ty ∈ entry.ancestors) ∧
+      InstanceOfEntityTags data entry
+-/
+/-
+def entitiesIsValid (env : Environment) (es : PartialEntities) : Bool :=
+  (es.toList.all entityIsValid) && (env.acts.toList.all instanceOfActionSchema)
+where
+  entityIsValid p :=
+    let (uid, ⟨attrs, ancestors, tags⟩) := p
+    match env.ets.find? uid.ty with
+    | .some entry =>
+      entry.isValidEntityEID uid.eid &&
+      (partialIsValid ancestors λ ancestors =>
+        ancestors.all (λ ancestor =>
+        entry.ancestors.contains ancestor.ty &&
+        instanceOfEntityType ancestor ancestor.ty env.ets.entityTypeMembers?)) &&
+      (partialIsValid attrs (instanceOfType · (.record entry.attrs) env.ets)) &&
+      (partialIsValid tags λ tags =>
+        match entry.tags? with
+        | .some tty => tags.values.all (instanceOfType · tty env.ets)
+        | .none     => tags == Map.empty)
+    | .none       => false
+  instanceOfActionSchema p :=
+    let (uid, entry) := p
+    match es.find? uid with
+    | .some entry₁ => entry.ancestors == entry₁.ancestors
+    | _            => false
+-/
+def PartialEntitiesMatchEnvironment (env : Environment) (entities: PartialEntities) : Prop :=
+  ∀ uid data, entities.find? uid = some data →
+    ∃ entry, env.ets.find? uid.ty = some entry ∧
+      IsValidEntityEID entry uid.eid ∧
+      PartialIsValid (InstanceOfType · (.record entry.attrs)) data.attrs ∧
+      PartialIsValid (λ ancestors => ∀ ancestor, ancestor ∈ ancestors → ancestor.ty ∈ entry.ancestors) data.ancestors ∧
+      PartialIsValid (InstanceOfEntityTags · entry) data.tags
 
 def PartialRequestAndEntitiesMatchEnvironment (env : Environment) (request : PartialRequest) (entities : PartialEntities) : Prop := sorry
 
 def IsConsistent (env : Environment) (req₁ : Request) (es₁ : Entities) (req₂ : PartialRequest) (es₂ : PartialEntities) : Prop := sorry
 
+theorem partial_request_matches_environment (env : Environment) (request : PartialRequest) :
+  requestIsValid env request → PartialRequestMatchesEnvironment env request
+:= by
+  intro h₁
+  simp [requestIsValid] at h₁
+  rcases h₁ with ⟨⟨h₁, h₂⟩, h₃⟩
+  simp [PartialRequestMatchesEnvironment]
+  apply And.intro
+  · exact partial_is_valid_rfl
+      (fun x =>
+    instanceOfEntityType x env.reqty.principal env.ets.entityTypeMembers?)
+      (fun x => InstanceOfEntityType x env.reqty.principal)
+      request.principal.asEntityUID
+      (λ x => @instance_of_entity_type_refl x env.reqty.principal env.ets.entityTypeMembers?) h₁
+  · apply And.intro
+    · exact partial_is_valid_rfl
+        (fun x =>
+      instanceOfEntityType x env.reqty.resource env.ets.entityTypeMembers?)
+        (fun x => InstanceOfEntityType x env.reqty.resource)
+        request.resource.asEntityUID
+        (λ x => @instance_of_entity_type_refl x env.reqty.resource env.ets.entityTypeMembers?) h₂
+    · have h₄ := partial_is_valid_rfl
+        (fun x => instanceOfType (Value.record x) (CedarType.record env.reqty.context) env.ets)
+        (fun x => InstanceOfType x (CedarType.record env.reqty.context))
+        request.context
+        (λ x => @instance_of_type_refl (Value.record x) (CedarType.record env.reqty.context) env.ets) h₃
+      simp [Option.bind]
+      split
+      · constructor
+      · rename_i heq
+        rw [heq] at h₄
+        simp only
+        cases h₄
+        rename_i heq
+        constructor
+        exact heq
+
+theorem partial_entities_match_environment (env : Environment) (entities : PartialEntities) :
+  entitiesIsValid env entities → PartialEntitiesMatchEnvironment env entities
+:= by sorry
 end Cedar.Thm
